main/SortingFun_common.v
@@ -1,0 +1,62 @@
+Set Nested Proofs Allowed.
+
+Require Import Utf8 Arith.
+Import List.ListNotations.
+(*
+Import Init.Nat.
+*)
+
+Require Import Misc PermutationFun.
+
+(* relation properties *)
+
+Definition irreflexive {A} (rel : A → A → bool) :=
+  ∀ a, rel a a = false.
+
+Definition antisymmetric {A} (rel : A → A → bool) :=
+  ∀ a b, rel a b = true → rel b a = true → a = b.
+
+(* https://ncatlab.org/nlab/show/connected+relation *)
+Definition connected_relation {A} (rel : A → A → bool) :=
+  ∀ a b, rel a b = false → rel b a = false → a = b.
+
+Definition transitive {A} (rel : A → A → bool) :=
+  ∀ a b c, rel a b = true → rel b c = true → rel a c = true.
+
+Definition total_relation {A} (rel : A → _) := ∀ a b,
+  (rel a b || rel b a)%bool = true.
+
+Theorem total_relation_is_reflexive : ∀ {A} {rel : A → _},
+  total_relation rel → reflexive rel.
+Proof.
+intros * Htot a.
+specialize (Htot a a) as H1.
+apply Bool.orb_true_iff in H1.
+now destruct H1.
+Qed.
+
+(* compute if a list is sorted *)
+
+Fixpoint is_sorted {A} (rel : A → A → bool) l :=
+  match l with
+  | [] => true
+  | [a] => true
+  | a :: (b :: _) as la => (rel a b && is_sorted rel la)%bool
+  end.
+
+Fixpoint all_sorted {A} (rel : A → A → bool) a l :=
+  match l with
+  | [] => true
+  | b :: l' => (rel a b && all_sorted rel a l')%bool
+  end.
+
+Fixpoint is_strongly_sorted {A} (rel : A → A → bool) l :=
+  match l with
+  | [] => true
+  | a :: l' => (all_sorted rel a l' && is_strongly_sorted rel l')%bool
+  end.
+
+Definition sorted {A} (rel : A → _) l :=
+  is_sorted rel l = true.
+Definition strongly_sorted {A} (rel : A → _) l :=
+  is_strongly_sorted rel l = true.
